pk_dh_game.v
@@ -2,7 +2,7 @@ From stdpp Require Import base gmap.
 From mathcomp Require Import ssreflect.
 From stdpp Require Import namespaces.
 From iris.algebra Require Import agree auth csum gset gmap excl frac.
-From iris.algebra Require Import numbers.
+From iris.algebra Require Import numbers reservation_map.
 From iris.heap_lang Require Import notation proofmode adequacy.
 From iris.heap_lang.lib Require Import par.
 From cryptis Require Import lib term cryptis primitives tactics.
@@ -24,10 +24,8 @@ Definition N := nroot.@"nsldh".
 
 Definition game : val := λ: "mkchan",
   let: "c"  := "mkchan" #() in
-  let: "nI" := mknonce #() in
-  let: "nR" := mknonce #() in
-  let: "kI" := mkkey (tag (nroot.@"key") "nI") in
-  let: "kR" := mkkey (tag (nroot.@"key") "nR") in
+  let: "kI" := mkakey #() in
+  let: "kR" := mkakey #() in
   let: "pkI" := Fst "kI" in
   let: "skI" := Snd "kI" in
   let: "pkR" := Fst "kR" in
@@ -51,45 +49,47 @@ Definition game : val := λ: "mkchan",
           eq_term "sesskI" "sesskR" && ~ eq_term "m" "sesskI")
   else SOME #true.
 
+(* MOVE *)
+#[global]
+Instance namespace_map_data_core_id {A : cmra} N (a : A) :
+  CoreId a → CoreId (namespace_map_data N a).
+Proof. apply _. Qed.
+(* /MOVE *)
+
 Lemma wp_game (mkchan : val) :
   {{{ True }}} mkchan #() {{{ v, RET v; channel v }}} -∗
+  cryptis_ctx -∗
   enc_pred_token ⊤ -∗
   key_pred_token (⊤ ∖ ↑nroot.@"keys") -∗
   nown_token session_name ⊤ -∗
+  ●H ∅ -∗
   WP game mkchan {{ v, ⌜v = NONEV ∨ v = SOMEV #true⌝ }}.
 Proof.
-iIntros "wp_mkchan enc_tok key_tok nown_tok"; rewrite /game; wp_pures.
+iIntros "wp_mkchan #ctx enc_tok key_tok nown_tok hon"; rewrite /game; wp_pures.
+iMod (own_alloc (reservation_map_token ⊤)) as (γI) "tokenI".
+  apply reservation_map_token_valid.
+iMod (own_alloc (reservation_map_token ⊤)) as (γR) "tokenR".
+  apply reservation_map_token_valid.
 pose (P rl (kI kR kS : term) :=
-  (∃ k, ⌜(if rl is Init then kI else kR) =
-         Spec.tag (nroot.@"key") k⌝ ∧
-        nonce_meta k (nroot.@"nsl") (kI, kR, kS))%I).
-iMod (pk_dh_alloc N P with "nown_tok enc_tok") as "[#ctx _]" => //.
-iMod (key_pred_set (nroot.@"key") (λ kt _, ⌜kt = Enc⌝)%I with "key_tok")
-  as "[#? _]" => //; try solve_ndisj.
+  own (if rl is Init then γI else γR)
+    (namespace_map_data nroot (to_agree (encode (kI, kR, kS))))).
+iMod (pk_dh_alloc N P with "nown_tok enc_tok") as "[#dh_ctx _]" => //.
+(* FIXME: This unshelve shouldn't be needed *)
+Unshelve. 2: apply _.
+(* /FIXME *)
 wp_bind (mkchan _); iApply "wp_mkchan" => //.
 iIntros "!> %c #cP".
-wp_pures; wp_bind (mknonce _).
-iApply (wp_mknonce (λ kI, nonce_meta kI (nroot.@"pub") ()) (λ _, False%I)).
-iIntros (kI) "#t_kI #p_kI _ tok_kI".
-wp_pures; wp_bind (mknonce _).
-iApply (wp_mknonce (λ _, nonce_meta kI (nroot.@"pub") ()) (λ _, False%I)).
-iIntros (kR) "#t_kR #p_kR _ tok_kR".
-rewrite (term_meta_token_difference kI (↑nroot.@"pub") ⊤) //.
-iDestruct "tok_kI" as "[pub init]".
-rewrite (term_meta_token_difference kR (↑nroot.@"pub") ⊤) //.
-iDestruct "tok_kR" as "[_ resp]".
-wp_pures; wp_tag; wp_bind (mkkey _); iApply wp_mkkey.
-set pkI := TKey Enc _.
-set skI := TKey Dec _.
-wp_pures; wp_tag; wp_bind (mkkey _); iApply wp_mkkey.
-set pkR := TKey Enc _.
-set skR := TKey Dec _.
+wp_pures; wp_bind (mkakey _).
+iApply (wp_mkakey with "[] [hon]"); eauto.
+iIntros "%kI #p_kI hon". wp_pures.
+wp_bind (mkakey _). iApply (wp_mkakey with "[] [hon]"); eauto.
+iIntros "%kR #p_kR hon". wp_pures.
+set pkI := TKey Enc kI.
+set skI := TKey Dec kI.
+set pkR := TKey Enc kR.
+set skR := TKey Dec kR.
 wp_pures; wp_bind (send _ _); iApply wp_send => //.
-  rewrite pterm_TKey sterm_tag; iRight; iSplit => //.
-  iExists _, _, _; eauto.
 wp_pures; wp_bind (send _ _); iApply wp_send => //.
-  rewrite pterm_TKey sterm_tag; iRight; iSplit => //.
-  iExists _, _, _; eauto.
 wp_pures; wp_bind (recv _); iApply wp_recv => //.
 iIntros (pkR') "#p_pkR'".
 wp_pures; wp_bind (is_key _); iApply wp_is_key.
@@ -98,114 +98,89 @@ wp_pures.
 case: bool_decide_reflect => [ekt|_]; last by wp_pures; iLeft.
 wp_pures; wp_bind (par _ _).
 case: kt epkR' ekt => // -> _.
+rewrite -Qp_half_half -dfrac_op_own. iDestruct "hon" as "[hon1 hon2]".
 iApply (wp_par (λ v, ∃ a : option term, ⌜v = repr a⌝ ∗ _)%I
                (λ v, ∃ a : option (term * term), ⌜v = repr a⌝ ∗ _)%I
-          with "[init] [resp]").
-- iApply (wp_pk_dh_init with "[//] [//] [] [] [init]") => //.
-  + rewrite [pterm (TKey Enc (Spec.tag _ _))]pterm_TKey sterm_tag.
-    iRight; iSplit => //.
-    iExists _, _, _; eauto.
-  + iIntros "%nI %nR".
+          with "[tokenI hon1] [tokenR hon2]").
+- iApply (wp_pk_dh_init with "[//] [//] [//] [] [] [tokenI hon1]") => //.
+  + iFrame. iIntros "%nI %nR".
     set (kS := mk_session_key _ _ _).
-    set (kI' := Spec.tag _ _).
-    iMod (term_meta_set _ _ (kI', kR', kS) (nroot.@"nsl") with "init").
-      solve_ndisj.
-    iModIntro. iExists _. by iFrame.
+    iMod (own_update with "tokenI").
+    * apply (namespace_map_alloc_update _ nroot
+               (to_agree (encode (kI, kR', kS)))) => //;
+      eauto.
+    * eauto.
   + iIntros "!> %a H". iExists a. iSplit; first done.
     iApply "H".
-- iApply (wp_pk_dh_resp with "[//] [//] [] [resp]") => //.
-  + rewrite [pterm (TKey Enc (Spec.tag _ _))]pterm_TKey sterm_tag.
-    iRight; iSplit => //.
-    iExists _, _, _; eauto.
-  + iIntros "%kI' %nI %nR".
+- iApply (wp_pk_dh_resp with "[//] [//] [//] [] [tokenR hon2]") => //.
+  + iFrame. iIntros "%kI' %nI %nR".
     set (kS := mk_session_key _ _ _).
-    set (kR'' := Spec.tag _ _).
-    iMod (term_meta_set _ _ (kI', kR'', kS) (nroot.@"nsl") with "resp").
-      solve_ndisj.
-    iModIntro. iExists _. by iFrame.
+    iMod (own_update with "tokenR").
+    * apply (namespace_map_alloc_update _ nroot
+               (to_agree (encode (kI', kR, kS)))) => //;
+      eauto.
+    * eauto.
   + iIntros "!> %a H"; iExists a; iSplit; first done.
     iApply "H".
 iIntros (v1 v2) "[H1 H2]".
-iDestruct "H1" as (a) "[-> H1]".
-iDestruct "H2" as (b) "[-> H2]".
-iModIntro; wp_pures.
+iDestruct "H1" as (a) "[-> [hon1 H1]]".
+iDestruct "H2" as (b) "[-> [hon2 H2]]".
+iCombine "hon1 hon2" as "hon". rewrite dfrac_op_own Qp_half_half.
+iModIntro.
+iMod (compromise_honest with "ctx hon") as "[hon comp]" => //.
+wp_pures.
+iMod "comp" as "#comp".
 case: a => [gabI|]; wp_pures; last by eauto.
 case: b => [[pkI' gabR]|]; wp_pures; last by eauto.
 iDestruct "H1" as "(#s_gabI & #confI & H1)".
 iDestruct "H2" as (kI') "(-> & #p_pkI' & #gabR & #confR & H2)".
-iAssert ((nonce_meta kI (nroot.@"pub") () → False) ∧
-         |==> nonce_meta kI (nroot.@"pub") ())%I with "[pub]" as "pub"; first iSplit.
-- iIntros "#contra".
-  by iApply (term_meta_meta_token with "pub contra").
-- by iApply (term_meta_set with "pub"); eauto.
-wp_eq_term e_pkR; wp_pures.
-  case: e_pkR => <- {kR'}.
-  iDestruct "H1" as "[#[contra|contra]|H1]".
-  - rewrite [pterm (TKey Dec _)]pterm_TKey pterm_tag.
-    iDestruct "contra" as "[contra|[_ contra]]".
-      iSpecialize ("p_kI" with "contra").
-      iAssert (▷ False)%I with "[pub]" as ">[]".
-      iModIntro.
-      by iDestruct "pub" as "[pub _]"; iApply "pub"; eauto.
-    by iMod (wf_key_elim with "contra [//]") as "%".
-  - rewrite [pterm (TKey Dec _)]pterm_TKey pterm_tag.
-    iDestruct "contra" as "[contra|[_ contra]]".
-      iSpecialize ("p_kR" with "contra").
-      iAssert (▷ False)%I with "[pub]" as ">[]".
-      by iDestruct "pub" as "[pub _]"; iApply "pub"; eauto.
-    by iMod (wf_key_elim with "contra [//]") as "%".
-  iDestruct "pub" as "[_ >#pub]".
-  wp_bind (send _ _); iApply wp_send => //.
-    rewrite [pterm skI]pterm_TKey pterm_tag; iModIntro.
-    iLeft; iApply "p_kI"; eauto.
-  wp_pures; wp_bind (send _ _); iApply wp_send => //.
-    rewrite [pterm skR]pterm_TKey pterm_tag; iModIntro.
-    iLeft; iApply "p_kR"; eauto.
-  iDestruct "H1" as "(#p_gabI & token & #sess)".
-  iPoseProof (session_key_confirmation _ Resp with "sess") as "confR'".
-  iDestruct "confR" as (k) "[%conf confR]".
-  case/Spec.tag_inj: conf => [_ <- {k}].
-  iDestruct "confR'" as (k) "[%conf confR']".
-  case/Spec.tag_inj: conf => [_ <- {k}] /=.
-  iPoseProof (term_meta_agree with "confR confR'") as "%valid".
-  case: valid => -> -> {kI' gabR}.
-  wp_pures.
-  wp_bind (recv _); iApply wp_recv => //; iIntros (m) "#p_m".
-  wp_pures; wp_bind (eq_term _ _); iApply wp_eq_term.
-  rewrite bool_decide_decide decide_True //.
-  wp_pures; wp_bind (eq_term _ _); iApply wp_eq_term.
-  rewrite bool_decide_decide decide_True //.
-  wp_pures; wp_bind (eq_term _ _); iApply wp_eq_term.
-  rewrite bool_decide_decide decide_True //.
-  case: (decide (m = gabI)) => [->|ne].
-    by iDestruct ("p_gabI" with "p_m") as ">[]".
-  wp_pures; wp_bind (eq_term _ _); iApply wp_eq_term.
-  rewrite bool_decide_decide decide_False //.
-  wp_pures; eauto.
-wp_eq_term e_pkI; wp_pures; last by eauto.
-case: e_pkI => <- {kI'}.
-iDestruct "H2" as "[[#contra|#contra]|H2]".
-- rewrite [pterm (TKey Dec _)]pterm_TKey pterm_tag.
-  iDestruct "contra" as "[contra|[_ contra]]".
-    iSpecialize ("p_kI" with "contra").
-    iAssert (▷ False)%I with "[pub]" as ">[]".
-    iModIntro.
-    iDestruct "pub" as "[pub _]"; iApply "pub"; eauto.
-  by iMod (wf_key_elim with "contra [//]") as "%".
-- rewrite [pterm (TKey Dec _)]pterm_TKey pterm_tag.
-  iDestruct "contra" as "[contra|[_ contra]]".
-    iSpecialize ("p_kR" with "contra").
-    iAssert (▷ False)%I with "[pub]" as ">[]".
-    by iDestruct "pub" as "[pub _]"; iApply "pub"; eauto.
-  by iMod (wf_key_elim with "contra [//]") as "%".
-iDestruct "H2" as "(#p_gabR & token & #H2)".
-iPoseProof (session_key_confirmation _ Init with "H2") as "confI'".
-iDestruct "confI" as (k) "[%conf confI]".
-case/Spec.tag_inj: conf => [_ <- {k}].
-iDestruct "confI'" as (k) "[%conf confI']".
-case/Spec.tag_inj: conf => [_ <- {k}].
-iPoseProof (term_meta_agree with "confI confI'") as "%valid".
-by case: valid e_pkR => -> _ /(_ eq_refl) [].
+pose (b := bool_decide (pkR = TKey Enc kR' ∨ pkI = TKey Enc kI')).
+wp_bind (eq_term pkR _ || _)%E.
+iApply (wp_wand _ _ _ (λ v, ⌜v = #b⌝)%I with "[] [H1 H2]").
+{ wp_eq_term e_pkR; wp_pures.
+    iPureIntro. by rewrite /b bool_decide_decide decide_True //; eauto.
+  iApply wp_eq_term. iPureIntro. congr (# (LitBool _)).
+  apply bool_decide_ext. intuition congruence. }
+iIntros "% ->". rewrite {}/b.
+case: bool_decide_reflect => [succ|_]; last by wp_pures; eauto.
+iAssert (⌜kR' = kR⌝ ∗
+         ⌜kI' = kI⌝ ∗
+         ⌜gabI = gabR⌝ ∗
+         □ (pterm gabI → ◇ False))%I with "[H1 H2]" as "#finish".
+{ case: succ => - [<-].
+  - iClear "H2". rewrite decide_True; try set_solver.
+    iDestruct "H1" as "(#p_gabI & token & #sess)".
+    iPoseProof (session_key_confirmation _ Resp with "sess") as "confR'".
+    iPoseProof (own_valid_2 with "confR confR'") as "%valid".
+    rewrite -reservation_map_data_op reservation_map_data_valid in valid.
+    rewrite to_agree_op_valid_L in valid.
+    case: (encode_inj _ _ valid) => -> -> {kI' gabR valid}. by eauto.
+  - iClear "H1". rewrite decide_True; try set_solver.
+    iDestruct "H2" as "(#p_gabR & token & #sess)".
+    iPoseProof (session_key_confirmation _ Init with "sess") as "confI'".
+    iPoseProof (own_valid_2 with "confI confI'") as "%valid".
+    rewrite -reservation_map_data_op reservation_map_data_valid in valid.
+    rewrite to_agree_op_valid_L in valid.
+    case: (encode_inj _ _ valid) => -> -> {kR' gabI valid}. by eauto. }
+iDestruct "finish" as "(-> & -> & <- & #p_gabI) {H1 H2}".
+wp_pures. wp_bind (send _ _). iApply wp_send => //.
+  iModIntro. rewrite big_sepS_forall. iApply "comp".
+  iPureIntro; set_solver.
+wp_pures. wp_bind (send _ _). iApply wp_send => //.
+  iModIntro. rewrite big_sepS_forall. iApply "comp".
+  iPureIntro; set_solver.
+wp_pures. wp_bind (recv _); iApply wp_recv => //; iIntros (m) "#p_m".
+wp_pures; wp_bind (eq_term _ _); iApply wp_eq_term.
+rewrite bool_decide_decide decide_True //.
+wp_pures; wp_bind (eq_term _ _); iApply wp_eq_term.
+rewrite bool_decide_decide decide_True //.
+wp_pures; wp_bind (eq_term _ _); iApply wp_eq_term.
+rewrite bool_decide_decide decide_True //.
+case: (decide (m = gabI)) => [->|ne].
+  by iDestruct ("p_gabI" with "p_m") as ">[]".
+wp_pures; wp_bind (eq_term _ _); iApply wp_eq_term.
+rewrite bool_decide_decide decide_False //.
+by wp_pures; eauto.
 Qed.
 
 End Game.
@@ -224,8 +199,8 @@ move=> wp_mkchan.
 apply (adequate_result NotStuck _ _ (λ v _, v = NONEV ∨ v = SOMEV #true)).
 apply: heap_adequacy.
 iIntros (?) "?".
-iMod (cryptisG_alloc _) as (?) "(_ & enc_tok & key_tok & _)".
+iMod (cryptisG_alloc _) as (?) "(#ctx & enc_tok & key_tok & ? & hon)".
 iMod (sessionG_alloc _) as (?) "nown_tok".
-iApply (wp_game with "[] [enc_tok] [key_tok]") => //.
+iApply (wp_game with "[] ctx [enc_tok] [key_tok] [nown_tok] [hon]") => //.
 iApply wp_mkchan.
 Qed.
